\documentclass[12pt]{article}
\usepackage{color}
\usepackage[pdftex]{graphicx}
\usepackage{tikz}
\usepackage{enumerate}
\usepackage[margin=0.25in,footskip=0.25in]{geometry}
\usepackage[normalem]{ulem}
\usepackage{setspace}
\usepackage{fancyvrb}
\usepackage{upquote}
\usepackage{amsmath}
\usepackage{amssymb}
\begin{document}
\section{Derivative of dot product}
$
f, g : \mathbb{R} \rightarrow \mathbb{R}^3\\
f_x, f_y, f_z, g_x, g_y, g_z : \mathbb{R} \rightarrow \mathbb{R}\\
f'(t) = \left[\begin{matrix}
f_x'(t) & f_y'(t) & f_z'(t)
\end{matrix}\right]\\
f \cdot g : \mathbb{R} \rightarrow \mathbb{R}\\
(f \cdot g)(t) = f_x(t)*g_x(t) + f_y(t) * g_y(t) + f_z(t) * g_z(t)\\
\frac{d}{dt}(f \cdot g)(t) = \frac{d}{dt}(f_x(t)*g_x(t) + f_y(t) * g_y(t) + f_z(t) * g_z(t)) = \\
\frac{d}{dt}(f_x(t)*g_x(t)) + \frac{d}{dt}(f_y(t) * g_y(t)) + \frac{d}{dt}(f_z(t) * g_z(t)) = \\
(f_x'(t)*g_x(t) + f_x(t)g_x'(t)) + (f_y'(t)*g_y(t) + f_y(t)g_y'(t)) + (f_z'(t)*g_z(t) + f_z(t)g_z'(t)) = \\
(f_x'(t)*g_x(t) + f_y'(t)*g_y(t) + f_z'(t)*g_z(t)) + (f_x(t)g_x'(t) + f_y(t)g_y'(t) + f_z(t)g_z'(t)) = \\
(f' \cdot g)(t) + (f \cdot g')(t)
$
\section{Curvature}
$
f, f', f'' : \mathbb{R} \rightarrow \mathbb{R}^n\\
f'(t) = \frac{df}{dt}(t)\\
k_f : \mathbb{R} \rightarrow \mathbb{R}\\
k_f(t) = \frac{\sqrt{||f'(t)||^2||f''(t)||^2 - (f'(t)\cdot f''(t))^2}}{||f'(t)||^3} =
\frac{\sqrt{f'(t)\cdot f'(t) * f''(t)\cdot f''(t) - (f'(t)\cdot f''(t))^2}}{(f'(t)\cdot f'(t))^{\frac{3}{2}}}\\
k_f'(t) = \frac{d}{dt}\frac{\sqrt{f'(t)\cdot f'(t) * f''(t)\cdot f''(t) - (f'(t)\cdot f''(t))^2}}{(f'(t)\cdot f'(t))^{\frac{3}{2}}} = \frac{a'(t)b(t) - b'(t)a(t)}{b(t)^2}\\
a = (f'\cdot f' * f''\cdot f'' - (f'\cdot f'')^2)^{\frac{1}{2}}\\
c = \frac{1}{2}(f'\cdot f' * f''\cdot f'' - (f'\cdot f'')^2)^\frac{-1}{2}\\
a' = c(\frac{d}{dt}(f'\cdot f' * f''\cdot f'' - (f'\cdot f'')^2)) =\\
c(\frac{d}{dt}(f'\cdot f' * f''\cdot f'') - \frac{d}{dt}(f'\cdot f'')^2) =\\
c((f''\cdot f'')\frac{df'\cdot f'}{dt} + (f'\cdot f')\frac{df''\cdot f''}{dt}) - 2(f'\cdot f'')\frac{d}{dt}(f'\cdot f'')) =^?\\
c((f''\cdot f'')(f'\cdot f'' + f''\cdot f') + (f'\cdot f')(f''\cdot f''' + f''' \cdot f'') - 2(f'\cdot f'')(f'\cdot f''' + f''\cdot f''))=\\
c((f''\cdot f'')(2f'\cdot f'') + (f'\cdot f')(2f''\cdot f''') - 2(f'\cdot f'')(f'\cdot f''' + f''\cdot f'')) =\\
c(2(f''\cdot f'')(f'\cdot f'') + 2(f'\cdot f')(f''\cdot f''') - 2(f'\cdot f'')f'\cdot f''' - 2(f'\cdot f'')f''\cdot f''))
\\
b(t) = (f'(t)\cdot f'(t))^{\frac{3}{2}}\\
b' = \frac{d}{dt}(f'\cdot f')^\frac{3}{2} =
\frac{3}{2}(f'\cdot f')^\frac{1}{2}(\frac{df'\cdot f'}{dt}) =^?
\frac{3}{2}(f'\cdot f')^\frac{1}{2}(f''\cdot f' + f' \cdot f'') =
\frac{3}{2}(f'\cdot f')^\frac{1}{2}(2f' \cdot f'')\\
b' = 3(f'\cdot f')^\frac{1}{2}(f' \cdot f'')\\
$
\end{document}
